proof/SimMemInj.v
@@ -1,0 +1,305 @@
+Require Import CoqlibC.
+Require Import Memory.
+Require Import Values.
+Require Import Maps.
+Require Import Events.
+Require Import Globalenvs.
+Require Import AST.
+
+Require Import SimMem.
+
+Set Implicit Arguments.
+
+(* Copied from CRELLVM *)
+Inductive frozen (f_old f_new: meminj) (bound_src bound_tgt: block): Prop :=
+| frozen_intro
+    (NEW_IMPLIES_OUTSIDE:
+       forall b_src b_tgt delta
+              (NEW: f_old b_src = None /\ f_new b_src = Some(b_tgt, delta)),
+         <<OUTSIDE_SRC: (bound_src <= b_src)%positive>> /\ <<OUTSIDE_TGT: (bound_tgt <= b_tgt)%positive>>)
+.
+
+Remark inject_separated_frozen
+       f_old f_new m_src m_tgt
+  :
+    Events.inject_separated f_old f_new m_src m_tgt <->
+    frozen f_old f_new m_src.(Mem.nextblock) m_tgt.(Mem.nextblock)
+.
+Proof.
+  unfold Events.inject_separated in *.
+  unfold Mem.valid_block in *.
+  split; i.
+  - econs; eauto.
+    i. des.
+    hexploit H; eauto. i; des.
+    splits; xomega.
+  - inv H.
+    exploit NEW_IMPLIES_OUTSIDE; eauto.
+    i; des.
+    split; xomega.
+Qed.
+
+Lemma frozen_preserves_src
+      f_old f_new
+      (INJECT: inject_incr f_old f_new)
+      bound_src bound_tgt
+      (FROZEN: frozen f_old f_new bound_src bound_tgt)
+      b_src
+      (INSIDE: (b_src < bound_src)%positive)
+  :
+    <<PRESERVED: f_old b_src = f_new b_src>>
+.
+Proof.
+  inv FROZEN.
+  destruct (f_old b_src) eqn:T0; ss;
+    destruct (f_new b_src) eqn:T1; ss.
+  - destruct p, p0; ss.
+    exploit INJECT; eauto; []; i; des.
+    clarify.
+  - destruct p; ss.
+    exploit INJECT; eauto; []; i; des.
+    clarify.
+  - destruct p; ss.
+    exploit NEW_IMPLIES_OUTSIDE; eauto; []; i; des.
+    exfalso.
+    xomega.
+Qed.
+
+Lemma frozen_preserves_tgt
+      f_old f_new
+      (INJECT: inject_incr f_old f_new)
+      bound_src bound_tgt
+      (FROZEN: frozen f_old f_new bound_src bound_tgt)
+      b_tgt
+      (INSIDE: (b_tgt < bound_tgt)%positive)
+  :
+    <<PRESERVED: forall b_src delta (NOW: f_new b_src = Some (b_tgt, delta)),
+      <<OLD: f_old b_src = Some (b_tgt, delta)>> >>
+.
+Proof.
+  inv FROZEN.
+  ii.
+  destruct (f_old b_src) eqn:T; ss.
+  - destruct p; ss.
+    exploit INJECT; eauto; []; i; des.
+    clarify.
+  - exfalso.
+    exploit NEW_IMPLIES_OUTSIDE; eauto; []; i; des.
+    xomega.
+Qed.
+
+Lemma frozen_shortened
+      f_old f_new
+      bd_src0 bd_tgt0
+      (FROZEN: frozen f_old f_new bd_src0 bd_tgt0)
+      bd_src1 bd_tgt1
+      (SHORT_SRC: (bd_src1 <= bd_src0)%positive)
+      (SHORT_TGT: (bd_tgt1 <= bd_tgt0)%positive)
+  :
+    <<FROZEN: frozen f_old f_new bd_src1 bd_tgt1>>
+.
+Proof.
+  inv FROZEN.
+  econs; eauto.
+  ii. des.
+  hexploit NEW_IMPLIES_OUTSIDE; eauto; []; i; des. clear NEW_IMPLIES_OUTSIDE.
+  split; ss.
+  - red. etransitivity; eauto.
+  - red. etransitivity; eauto.
+Qed.
+
+Lemma frozen_refl
+      f
+      bound_src bound_tgt
+  :
+    <<FROZEN: frozen f f bound_src bound_tgt>>
+.
+Proof.
+  econs; eauto. i; des. clarify.
+Qed.
+
+
+
+Section MEMINJ.
+
+Local Existing Instance Val.mi_normal.
+(* Variable gbound_src gbound_tgt: block. *)
+
+Record t' := mkrelation {
+  inj: meminj; (* public memory injection *)
+  src_private: forall (b: block) (ofs: Z), Prop; (* source private memory *)
+  tgt_private: forall (b: block) (ofs: Z), Prop; (* target private memory *)
+  src_external: forall (b: block) (ofs: Z), Prop; (* source external memory *)
+  tgt_external: forall (b: block) (ofs: Z), Prop; (* target external memory *)
+  src_mem: mem; (* source memory *)
+  tgt_mem: mem; (* target memory *)
+  src_mem_parent: mem;
+  tgt_mem_parent: mem;
+}.
+
+Inductive wf' (rel: t'): Prop :=
+| wf_intro
+    (PUBLIC: Mem.inject rel.(inj) rel.(src_mem) rel.(tgt_mem))
+    (SRCDISJ: rel.(src_private) \2/ rel.(src_external) <2= loc_unmapped rel.(inj))
+    (TGTDISJ: rel.(tgt_private) \2/ rel.(tgt_external) <2= loc_out_of_reach rel.(inj) rel.(src_mem))
+    (SRCPRIVEXT: forall b ofs, ~ (rel.(src_private) b ofs /\ rel.(src_external) b ofs))
+    (TGTPRIVEXT: forall b ofs, ~ (rel.(tgt_private) b ofs /\ rel.(tgt_external) b ofs))
+    (SRCSUBSET: forall b ofs, rel.(src_private) b ofs \/
+                         rel.(src_external) b ofs ->
+                         Plt b rel.(src_mem).(Mem.nextblock))
+    (TGTSUBSET: forall b ofs, rel.(tgt_private) b ofs \/
+                         rel.(tgt_external) b ofs ->
+                         Plt b rel.(tgt_mem).(Mem.nextblock))
+    (SRCPBOUND: (rel.(src_mem_parent).(Mem.nextblock) <= rel.(src_mem).(Mem.nextblock))%positive)
+    (TGTPBOUND: (rel.(tgt_mem_parent).(Mem.nextblock) <= rel.(tgt_mem).(Mem.nextblock))%positive)
+    (* It should be mem_parent, in order to exploit "FROZEN" *)
+    (* (SRCGBOUND: (gbound_src <= rel.(src_mem_parent).(Mem.nextblock))%positive) *)
+    (* (TGTGBOUND: (gbound_tgt <= rel.(tgt_mem_parent).(Mem.nextblock))%positive) *)
+.
+
+Inductive le' (mrel0 mrel1: t'): Prop :=
+| le_intro
+    (INCR: inject_incr mrel0.(inj) mrel1.(inj))
+    (SRCEXT: mrel0.(src_external) <2= mrel1.(src_external))
+    (TGTEXT: mrel0.(tgt_external) <2= mrel1.(tgt_external))
+    (SRCUNCHANGED: Mem.unchanged_on mrel0.(src_external) mrel0.(src_mem) mrel1.(src_mem))
+    (TGTUNCHANGED: Mem.unchanged_on mrel0.(tgt_external) mrel0.(tgt_mem) mrel1.(tgt_mem))
+    (SRCPARENTEQ: mrel0.(src_mem_parent) = mrel1.(src_mem_parent))
+    (TGTPARENTEQ: mrel0.(tgt_mem_parent) = mrel1.(tgt_mem_parent))
+    (FROZEN: frozen mrel0.(inj) mrel1.(inj) (mrel0.(src_mem_parent).(Mem.nextblock))
+                                            (mrel0.(tgt_mem_parent).(Mem.nextblock)))
+    (SRCBOUND: (mrel0.(src_mem).(Mem.nextblock) <= mrel1.(src_mem).(Mem.nextblock))%positive)
+    (TGTBOUND: (mrel0.(tgt_mem).(Mem.nextblock) <= mrel1.(tgt_mem).(Mem.nextblock))%positive)
+.
+
+Definition lift' (mrel0: t'): t' :=
+  (mkrelation mrel0.(inj) (fun _ _ => False) (fun _ _ => False)
+                          (mrel0.(src_private) \2/ mrel0.(src_external))
+                          (mrel0.(tgt_private) \2/ mrel0.(tgt_external))
+                          mrel0.(src_mem) mrel0.(tgt_mem) mrel0.(src_mem) mrel0.(tgt_mem))
+.
+
+Definition unlift' (mrel0 mrel1: t'): t' :=
+  (mkrelation mrel1.(inj)
+                      (mrel0.(src_private)) (mrel0.(tgt_private))
+                      (mrel0.(src_external)) (mrel0.(tgt_external))
+                      mrel1.(src_mem) mrel1.(tgt_mem) mrel0.(src_mem_parent) mrel0.(tgt_mem_parent))
+.
+
+(* TODO: Let's have this as policy. (giving explicit name) *)
+(* TODO: apply this policy for identity/extension *)
+
+(* "Global" is needed as it is inside section *)
+Global Program Instance SimMemInj : SimMem.class :=
+{
+  t := t';
+  src_mem := src_mem;
+  tgt_mem := tgt_mem;
+  wf := wf';
+  le := le';
+  lift := lift';
+  unlift := unlift';
+  sim_val := fun (mrel: t') => Val.inject mrel.(inj);
+}.
+Next Obligation.
+  econs.
+  - i. econs; eauto; try reflexivity; try apply Mem.unchanged_on_refl; eauto.
+    { eapply frozen_refl; eauto. }
+  - ii. inv H; inv H0.
+    econs; eauto.
+    + eapply inject_incr_trans; eauto.
+    + eapply Mem.unchanged_on_implies in SRCUNCHANGED0.
+      eapply Mem.unchanged_on_trans; eauto.
+      i. eapply SRCEXT; eauto.
+    + eapply Mem.unchanged_on_implies in TGTUNCHANGED0.
+      eapply Mem.unchanged_on_trans; eauto.
+      i. eapply TGTEXT; eauto.
+    + rewrite SRCPARENTEQ. ss.
+    + rewrite TGTPARENTEQ. ss.
+    + econs; eauto.
+      ii; des.
+      destruct (inj y b_src) eqn:T.
+      * destruct p.
+        exploit INCR0; eauto. i; clarify.
+        inv FROZEN.
+        hexploit NEW_IMPLIES_OUTSIDE; eauto.
+      * inv FROZEN0.
+        hexploit NEW_IMPLIES_OUTSIDE; eauto; []; i; des.
+        split; ss.
+        rewrite SRCPARENTEQ. ss.
+        rewrite TGTPARENTEQ. ss.
+    + etransitivity; eauto.
+    + etransitivity; eauto.
+Qed.
+Next Obligation.
+  rename H into VALID.
+  inv VALID. econs; ss; eauto; ii; des; ss; eauto.
+  - eapply TGTDISJ; eauto.
+  - eapply TGTDISJ; eauto.
+  - eapply Pos.compare_gt_iff in H. xomega.
+  - eapply Pos.compare_gt_iff in H. xomega.
+  (* - eapply Pos.compare_gt_iff in H. xomega. *)
+  (* - eapply Pos.compare_gt_iff in H. xomega. *)
+Qed.
+Next Obligation.
+  inv H; ss.
+  econs; ss; eauto; ii; des; ss.
+  - eapply Mem.unchanged_on_implies; eauto.
+    i. right. ss.
+  - eapply Mem.unchanged_on_implies; eauto.
+    i. right. ss.
+  - inv H0. ss.
+    eapply frozen_shortened; eauto.
+Qed.
+Next Obligation.
+  inv H. inv H0. inv H1.
+  econs; ss; eauto. (* eauto did well here *)
+  - etransitivity; eauto.
+  - etransitivity; eauto.
+Qed.
+
+Lemma loc_unmapped_frozen
+      F F'
+      fbound_src fbound_tgt
+      (FROZEN : frozen F F' fbound_src fbound_tgt)
+      b ofs
+      (BOUND: Plt b fbound_src)
+      (UNMAPPED: loc_unmapped F b ofs)
+  :
+    loc_unmapped F' b ofs
+.
+Proof.
+  unfold loc_unmapped in *.
+  destruct (F' b) eqn:T; ss.
+  destruct p; ss.
+  inv FROZEN.
+  exploit NEW_IMPLIES_OUTSIDE; eauto.
+  i; des. xomega.
+Qed.
+
+Lemma loc_out_of_reach_frozen
+      F F'
+      fbound_src fbound_tgt
+      (INCR: inject_incr F F')
+      (FROZEN : frozen F F' fbound_src fbound_tgt)
+      b ofs
+      (BOUND: Plt b fbound_tgt)
+      m0 m1
+      (UNMAPPED: loc_out_of_reach F m0 b ofs)
+      (UNCHANGED: forall k p b0 delta (MAPPED: F b0 = Some (b, delta)),
+          Mem.perm m0 b0 (ofs - delta) k p <-> Mem.perm m1 b0 (ofs - delta) k p)
+  :
+    loc_out_of_reach F' m1 b ofs
+.
+Proof.
+  unfold loc_out_of_reach in *.
+  i.
+  exploit frozen_preserves_tgt; eauto.
+  i. des.
+  hexploit UNMAPPED; eauto. i.
+  ii.
+  contradict H1.
+  eapply UNCHANGED; eauto.
+Qed.
+
+End MEMINJ.
